code/ecdsap256/Hacl.P256.fsti
@@ -412,3 +412,14 @@ val getScalar: #buf_type: buftype -> scalar: lbuffer_t buf_type uint8 (size 32) 
   Stack uint32 
     (requires fun h -> True)
     (ensures fun h0 _ h1 -> True)
+
+
+val montgomery_ladder_step_radix:  #buf_type: buftype ->
+  p: point -> tempBuffer: lbuffer uint64 (size 88) -> 
+  t: lbuffer uint64 (size 8 *! size 16) ->
+  scalar: lbuffer_t buf_type uint8 (size 32) -> 
+  i:size_t{v i < 256} -> 
+  Stack unit
+  (requires fun h -> live h p /\live h tempBuffer /\ live h scalar /\
+    LowStar.Monotonic.Buffer.all_disjoint [loc p;loc tempBuffer; loc scalar])
+  (ensures fun h0 _ h1 -> True)
